Prove fullCaseXS

acl2/models.lisp
@@ -1,81 +1,83 @@
 (in-package "RTL")
 (include-book "ihs/basic-definitions" :dir :system)
 (include-book "kestrel/utilities/fixbytes/instances" :dir :system)
-(include-book "rtl/rel11/portcullis" :dir :system)
+(include-book "rtl/rel11/support/definitions" :dir :system)
 
 (include-book "tools/with-arith5-help" :dir :system)
 (local (acl2::allow-arith5-help))
 
+(local (include-book "rtl/rel11/support/basic" :dir :system))
+
 ; Coerce x to a signed integer which will fit in n bits.
 (acl2::with-arith5-help
- (acl2::define int-fix
+ (define int-fix
    ((x integerp))
    :returns (result acl2::sbyte32p
                     :hints (("goal" :in-theory (enable acl2::sbyte32p))))
    (acl2::logext 32 (ifix x))
    ///
    (fty::deffixequiv int-fix)
-   (acl2::defrule int-fix-type
+   (defrule int-fix-type
      (integerp (int-fix x))
      :rule-classes :type-prescription)
-   (acl2::defruled int-fix-when-sbyte32
+   (defrule int-fix-when-sbyte32
      (implies (acl2::sbyte32p x)
               (equal (int-fix x) x))
      :enable acl2::sbyte32p)))
 
 (acl2::with-arith5-help
- (acl2::define long-fix
+ (define long-fix
    ((x integerp))
    :returns (result acl2::sbyte64p
                     :hints (("goal" :in-theory (enable acl2::sbyte64p))))
    (acl2::logext 64 (ifix x))
    ///
    (fty::deffixequiv long-fix)
-   (acl2::defrule long-fix-type
+   (defrule long-fix-type
      (integerp (long-fix x))
      :rule-classes :type-prescription)
-   (acl2::defruled long-fix-when-sbyte64
+   (defrule long-fix-when-sbyte64
      (implies (acl2::sbyte64p x)
               (equal (long-fix x) x))
      :enable acl2::sbyte64p)))
 
-(acl2::defruled sbyte32-suff
+(defruled sbyte32-suff
   (implies (and (integerp x)
                 (<= #fx-1p31 x)
                 (< x #fx1p31))
            (acl2::sbyte32p x))
   :enable acl2::sbyte32p)
 
-(acl2::defruled sbyte64-suff
+(defruled sbyte64-suff
   (implies (and (integerp x)
                 (<= #fx-1p63 x)
                 (< x #fx1p63))
            (acl2::sbyte64p x))
   :enable acl2::sbyte64p)
 
-(acl2::defrule sbyte32-fix-type
+(defrule sbyte32-fix-type
   (integerp (acl2::sbyte32-fix x))
   :rule-classes :type-prescription
   :enable acl2::sbyte32-fix)
 
-(acl2::defrule sbyte64-fix-type
+(defrule sbyte64-fix-type
   (integerp (acl2::sbyte64-fix x))
   :rule-classes :type-prescription
   :enable acl2::sbyte64-fix)
 
-(acl2::defrule sbyte32-is-integer
+(defrule sbyte32-is-integer
   (implies (acl2::sbyte32p x)
            (integerp x)))
 
-(acl2::defrule sbyte64-is-integer
+(defrule sbyte64-is-integer
   (implies (acl2::sbyte64p x)
            (integerp x)))
 
-(acl2::defrule sbyte32-is-acl2-numberp
+(defrule sbyte32-is-acl2-numberp
   (implies (acl2::sbyte32p x)
            (acl2-numberp x)))
 
-(acl2::defrule sbyte64-is-acl2-numberp
+(defrule sbyte64-is-acl2-numberp
   (implies (acl2::sbyte64p x)
            (acl2-numberp x)))
 
@@ -90,13 +92,38 @@
    (and (not (= y 0)) (long-fix (truncate x y))))
   ///
   (fty::deffixequiv ldiv)
-  (defrule sbyte64-ldiv-noexcept
+  (defrule sbyte64p-ldiv-noexcept
     (implies (not (= (acl2::sbyte64-fix y) 0))
              (acl2::sbyte64p (ldiv x y))))
   (defrule ldiv-type-noexcept
     (implies (not (= (acl2::sbyte64-fix y) 0))
              (integerp (ldiv x y)))
-    :rule-classes :type-prescription))
+    :rule-classes :type-prescription)
+  (defruled ldiv-when-nonnegative-args
+    (implies (and (<= 0 (acl2::sbyte64-fix x))
+                  (< 0 (acl2::sbyte64-fix y)))
+             (equal (ldiv x y)
+                    (fl (/ (acl2::sbyte64-fix x) (acl2::sbyte64-fix y)))))
+    :use (:instance lemma
+                    (x (acl2::sbyte64-fix x))
+                    (y (acl2::sbyte64-fix y)))
+    :prep-lemmas
+    ((acl2::with-arith5-nonlinear-help
+      (defrule lemma
+        (implies (and (acl2::sbyte64p x)
+                      (acl2::sbyte64p y)
+                      (<= 0 x)
+                      (< 0 y))
+                 (equal (ldiv x y) (fl (/ x y))))
+        :enable (acl2::sbyte64p fl)))))
+  (acl2::with-arith5-help
+   (defrule ldiv-type-when-nonnegative-args
+     (implies (and (<= 0 (acl2::sbyte64-fix x))
+                   (< 0 (acl2::sbyte64-fix y)))
+              (natp (ldiv x y)))
+     :rule-classes :type-prescription
+     :disable ldiv
+     :use ldiv-when-nonnegative-args)))
 
 (define lrem
   ((x acl2::sbyte64p)
@@ -106,23 +133,42 @@
   (acl2::b*
    ((x (acl2::sbyte64-fix x))
     (y (acl2::sbyte64-fix y)))
-   (and (not (= y 0)) (long-fix (- x (* y (truncate x y))))))
+   (and (not (= y 0)) (long-fix (rem x y))))
   ///
   (fty::deffixequiv lrem)
-  (defrule sbyte64-lrem-noexcept
+  (defrule sbyte64p-lrem-noexcept
     (implies (not (= (acl2::sbyte64-fix y) 0))
              (acl2::sbyte64p (lrem x y))))
-  (defruled lrem-type-noexcept
+  (defrule lrem-type-noexcept
     (implies (not (= (acl2::sbyte64-fix y) 0))
              (integerp (lrem x y)))
     :rule-classes :type-prescription)
-  (defruled lrem-type-noexcept-corr
-    (implies (and (acl2::sbyte64p y)
-                  (not (= y 0)))
-             (integerp (lrem x y)))
-    :rule-classes :type-prescription))
+  (defruled lrem-when-nonnegative-args
+    (implies (and (<= 0 (acl2::sbyte64-fix x))
+                  (< 0 (acl2::sbyte64-fix y)))
+             (equal (lrem x y)
+                    (mod (acl2::sbyte64-fix x) (acl2::sbyte64-fix y))))
+    :use (:instance lemma
+                    (x (acl2::sbyte64-fix x))
+                    (y (acl2::sbyte64-fix y)))
+    :prep-lemmas
+    ((acl2::with-arith5-nonlinear-help
+      (defrule lemma
+        (implies (and (acl2::sbyte64p x)
+                      (acl2::sbyte64p y)
+                      (<= 0 x)
+                      (< 0 y))
+                 (equal (lrem x y) (mod x y)))
+        :enable acl2::sbyte64p))))
+  (acl2::with-arith5-help
+   (defrule lrem-type-when-nonnegative-args
+     (implies (and (<= 0 (acl2::sbyte64-fix x))
+                   (< 0 (acl2::sbyte64-fix y)))
+              (natp (lrem x y)))
+     :rule-classes :type-prescription
+     :use lrem-when-nonnegative-args)))
 
-(acl2::define Natural.compareTo
+(define Natural.compareTo
   ((this natp)
    (y natp))
   :returns (result acl2::sbyte32p)
@@ -132,12 +178,12 @@
    (signum (- this y)))
   ///
   (fty::deffixequiv Natural.compareTo)
-  (acl2::defrule Natural.compareTo-linear
+  (defrule Natural.compareTo-linear
     (and (<= -1 (Natural.compareTo this x))
          (<= (Natural.compareTo this x) 1))
     :rule-classes :linear))
 
-(acl2::define Natural.closerTo
+(define Natural.closerTo
   ((this natp)
    (x natp)
    (y natp))
@@ -149,13 +195,13 @@
    (signum (- (* 2 this) (+ x y))))
   ///
   (fty::deffixequiv Natural.closerTo)
-  (acl2::defrule Natural.closerTo-linear
+  (defrule Natural.closerTo-linear
     (and (<= -1 (Natural.closerTo this x y))
          (<= (Natural.closerTo this x y) 1))
     :rule-classes :linear))
 
 (acl2::with-arith5-help
- (acl2::define Natural.valueOfShiftLeft
+ (define Natural.valueOfShiftLeft
    ((v acl2::sbyte64p)
     (n acl2::sbyte32p))
    :returns (result-or-exception (or (null result-or-exception)
@@ -169,12 +215,12 @@
     (ash unsigned-v n))
    ///
    (fty::deffixequiv Natural.valueOfShiftLeft)
-   (acl2::defrule Natural.valueOfShiftLeft-type-noexception
+   (defrule Natural.valueOfShiftLeft-type-noexception
      (implies (<= 0 (acl2::sbyte32-fix n))
               (natp (Natural.valueOfShiftLeft v n)))
      :rule-classes :type-prescription)
    (acl2::with-arith5-nonlinear-help
-    (acl2::defrule Natural.valueOfShiftLeft-when-nonnegative
+    (defrule Natural.valueOfShiftLeft-when-nonnegative
       (implies (and (<= 0 (acl2::sbyte64-fix v))
                     (<= 0 (acl2::sbyte32-fix n)))
                (equal (Natural.valueOfShiftLeft v n)
@@ -183,7 +229,7 @@
      :enable (acl2::sbyte64-fix acl2::sbyte64p)))))
 
 (acl2::with-arith5-help
- (acl2::define gen-powers
+ (define gen-powers
    ((b integerp)
     (n natp))
    :returns (powers acl2::sbyte64-listp)
@@ -200,7 +246,7 @@
 (defconst *Powers.pow10*
   (gen-powers 10 (+ *Powers.MAX_POW_10_EXP* 1)))
 
-(acl2::defruled nth-pow10-when-i<=MAX_POW_10_EXP
+(defruled nth-pow10-when-i<=MAX_POW_10_EXP
   (implies (and (natp i)
                 (< i (len *Powers.pow10*)))
            (equal (nth i *Powers.pow10*)
@@ -210,7 +256,7 @@
           (= i 10) (= i 11) (= i 12) (= i 13) (= i 14)
           (= i 15) (= i 16) (= i 17) (= i 18) (= i 19)))
 
-(acl2::define Powers.pow10[]
+(define Powers.pow10[]
   ((i acl2::sbyte32p))
   :returns (result-or-exception (implies result-or-exception
                                          (acl2::sbyte64p result-or-exception))
@@ -220,18 +266,18 @@
    (and (natp i) (< i (len *Powers.pow10*)) (nth i *Powers.pow10*)))
   ///
   (fty::deffixequiv Powers.pow10[])
-  (acl2::defrule Powers.pow10[]-type
+  (defrule Powers.pow10[]-type
     (or (null (Powers.pow10[] i))
         (integerp (Powers.pow10[] i)))
     :rule-classes :type-prescription)
-  (acl2::defruled Powers.pow10[]-when-i<=MAX_POW_10_EXP
+  (defruled Powers.pow10[]-when-i<=MAX_POW_10_EXP
     (implies (and (natp i)
                   (<= i *Powers.MAX_POW_10_EXP*))
              (equal (Powers.pow10[] i)
                     (long-fix (expt 10 i))))
     :enable acl2::sbyte32p
     :use (:instance nth-pow10-when-i<=MAX_POW_10_EXP))
-  (acl2::defruled Powers.pow10[]-when-i<MAX_POW_10_EXP
+  (defruled Powers.pow10[]-when-i<MAX_POW_10_EXP
     (implies (and (natp i)
                   (< i *Powers.MAX_POW_10_EXP*))
              (equal (Powers.pow10[] i)
@@ -256,7 +302,7 @@
 ; stub of method DoubleToDecimal.toChars(long f, int e)
 ; returns positive rational instead of String
 ; TODO implement rendering to chars
-(acl2::define DoubleToDecimal.toChars
+(define DoubleToDecimal.toChars
   ((this DoubleToDecimal-p)
    (f acl2::sbyte64p)
    (e acl2::sbyte32p))
@@ -268,262 +314,17 @@
    (* f (expt 10 (- e *H*))))
   ///
   (fty::deffixequiv DoubleToDecimal.toChars))
-;  (acl2::with-arith5-help
-;   (acl2::defrule DoubleToDecimal.toChars-type-noexception
-;     (implies (< 0 (acl2::sbyte64-fix f))
-;              (rtl::pos-rationalp (DoubleToDecimal.toChars this f e)))
-;     :rule-classes :type-prescription)))
-#|
-(local
- (acl2::with-arith5-help
-  (defrule mod-sbH-lemma
-    (implies (and (acl2::sbyte64p sbH)
-                  (<= 0 sbH)
-                  (posp di))
-             (acl2::sbyte64p (mod sbH di)))
-    :enable acl2::sbyte64p)))
 
 (local
  (acl2::with-arith5-help
-  (defrule mod-sbH-lemma-2
-    (implies (and (acl2::sbyte64p sbH)
-                  (<= 0 sbH)
-                  (posp di))
-             (acl2::sbyte64p (- sbH (mod sbH di))))
-    :enable acl2::sbyte64p)))
-
-(local
- (acl2::with-arith5-nonlinear-help
-  (defrule mod-sbH-lemma-3
-    (implies (and (acl2::sbyte64p sbH)
-                  (<= 0 sbH)
-                  (< sbH (expt (D) *H*))
-                  (posp di)
-                  (<= di (expt (D) *H*))
-                  )
-             (acl2::sbyte64p (+ sbH
-                                di
-                                (- (mod sbH di)))))
-    :enable (acl2::sbyte64p (D)))))
-
-(local
- (defrule --g-lemma
-   (implies (and (acl2::sbyte32p g)
-                 (<= 0 g))
-            (acl2::sbyte32p (1- g)))
-   :enable acl2::sbyte32p
-   ))
-
-(define v-dp
-  ((this DoubleToDecimal-p))
-  :returns (v (finite-positive-binary-p v (dp))
-              :hints (("goal" :in-theory (enable (dp)))))
-  (acl2::b*
-   (((DoubleToDecimal this) this)
-    (v (* this.c (expt 2 this.q))))
-   (if (finite-positive-binary-p v (dp)) v 1))
-  ///
-  (fty::deffixequiv v-dp))
-
-(define i-dp
-  ((g acl2::sbyte32p))
-  :returns (i posp :rule-classes :type-prescription)
-  (acl2::b*
-   ((g (acl2::sbyte32-fix g)))
-   (if (and (<= 0 g)
-            (< g *H*))
-       (- *H* g)
-     *H*))
-  ///
-  (fty::deffixequiv i-dp)
-  (defrule i-dp-linear
-    (<= (i-dp g) (H (dp)))
-    :rule-classes :linear
-    :enable ((dp))))
-
-(acl2::with-arith5-help
- (defruled s_i-as-!s_i
-   (implies (and (natp hi)
-                 (< hi (H (dp))))
-            (equal (- (s_i (H (dp)) v)
-                      (acl2::sbyte64-fix (mod (s_i (H (dp)) v) (expt (D) hi))))
-                   (!s_i (- (H (dp)) hi) v (dp))))
-   :disable mod
-   :expand (!s_i (H (dp)) v (dp))
-   :use ((:instance !s_i-as-!s_H
-                    (f (dp))
-                    (i (- (H (dp)) hi)))
-         (:instance mod-def
-                    (x (!s_i (H (dp)) v (dp)))
-                    (y (expt (D) hi))))
-   :prep-lemmas
-   ((defrule lemma
-      (implies (and (integerp hi)
-                    (natp sh)
-                    (natp hi)
-                    (< hi (H (dp))))
-               (acl2::sbyte64p (mod sh (expt (D) hi))))
-      :enable (acl2::sbyte64p (D) (dp))
-      :use (:instance mod-bnd-1
-                      (m sh)
-                      (n (expt (D) hi)))))))
-
-(acl2::with-arith5-nonlinear-help
- (defruled sbyte64p-!s_i
-   (acl2::sbyte64p (!s_i i v (dp)))
-   :enable (!s_i acl2::sbyte64p (dp) (D))
-   :use (:instance s_i-linear
-                   (i (min (H (dp)) (acl2::pos-fix i))))))
-
-(acl2::with-arith5-help
- (defruled !s-i+D^{H-i}-as-!t_i
-   (implies (and (<= (acl2::pos-fix i) (H f))
-                 (= hi (- (H f) (acl2::pos-fix i)))
-                 )
-            (equal (+ (expt (D) hi) (!s_i i v f))
-                   (!t_i i v f)))
-   :enable (!s_i !t_i t_i)))
-|#
-#|
-(acl2::with-arith5-help
- (define DoubleToDecimal.fullCaseXS-loop-invariant
-   ((this DoubleToDecimal-p)
-    (g acl2::sbyte32p)
-    (sbH acl2::sbyte64p)
-    (p acl2::sbyte32p)
-    (vb natp)
-    (vbl natp)
-    (vbr natp))
-   :returns (yes booleanp :rule-classes ())
-   (acl2::b*
-    (((DoubleToDecimal this) this)
-     (f (dp))
-     (H (H f))
-     ((unless (posp this.c)) nil)
-     (v (* this.c (expt 2 this.q)))
-     (e (e v))
-     (!q (!q v f)))
-    (and
-     (<= (Qmin f) this.q)
-     (<= this.q (Qmax f))
-     (or (= this.q (Qmin f)) (<= (2^{P-1} f) this.c))
-     (<= this.c (Cmax f))
-     (natp g)
-     (< g H)
-     (finite-positive-binary-p v f)
-     (= sbH (!s_i H v f))
-     (<= 0 p)
-     (<= e H)
-     (= p (- e (+ H !q)))
-     (= vb (vb v f))
-     (= vbl (vbl v f))
-     (= vbr (vbr v f))
-     ))
-   ///
-   (defrule DoubleToDecimal.fullCaseXS-loop-invariant-fwd
-     (implies (DoubleToDecimal.fullCaseXS-loop-invariant
-               this g sbH p vb vbl vbr)
-              (let ((f (dp))
-                    (v (v-dp this)))
-                (and (natp g)
-                     (< g (H f))
-                     (finite-positive-binary-p v f)
-                     (= sbH (!s_i (H f) v f))
-                     (= p (- (e v) (+ (H f) (!q v f))))
-                     (= vb (vb v f))
-                     (= vbl (vbl v f))
-                     (= vbr (vbr v f)))))
-     :rule-classes :forward-chaining
-     :enable (v-dp Cmax)
-     :use (:instance finite-positive-binary-suff
-                     (f (dp))
-                     (q (DoubleToDecimal->q this))
-                     (c (DoubleToDecimal->c this))))
-   (defrule i-dp-type-when-DoubleToDecimal.fullCaseXS-loop-invariant
-     (implies (DoubleToDecimal.fullCaseXS-loop-invariant
-               this g sbH p vb vbl vbr)
-              (posp (i-dp g)))
-     :rule-classes :type-prescription)
-   (defrule i-dp-linear-when-DoubleToDecimal.fullCaseXS-loop-invariant
-     (implies (DoubleToDecimal.fullCaseXS-loop-invariant
-               this g sbH p vb vbl vbr)
-              (<= (i-dp g) (H (dp))))
-     :rule-classes :linear)
-   (defrule v-dp-when-DoubleToDecimal.fullCaseXS-loop-invariant
-     (implies (DoubleToDecimal.fullCaseXS-loop-invariant
-               this g sbH p vb vbl vbr)
-              (finite-positive-binary-p (v-dp this) (dp)))
-     :enable DoubleToDecimal.fullCaseXS-loop-invariant-fwd)
-   (defrule Power.pow10[]-g-when-DoubleToDecimal.fullCaseXS-loop-invariant
-     (implies (DoubleToDecimal.fullCaseXS-loop-invariant
-                    this g sbH p vb vbl vbr)
-              (equal (Powers.pow10[] g)
-                     (expt (D) (- (H (dp)) (i-dp g)))))
-     :enable (i-dp (dp))
-     :use (:instance Powers.pow10[]-when-i<MAX_POW_10_EXP
-                     (i (acl2::sbyte32-fix g))))
-   #|
-   (defrule sbyte64-fix-sbH-when-DoubleToDecimal.fullCaseXS-loop-invariant
-     (implies (DoubleToDecimal.fullCaseXS-loop-invariant
-                    this g sbH p vb vbl vbr)
-              (equal (acl2::sbyte64-fix sbH)
-                     (s_i (H (dp)) (v-dp this))))
-     :enable v-dp)
-   (defrule sbyte32-fix-p-when-DoubleToDecimal.fullCaseXS-loop-invariant
-     (implies (DoubleToDecimal.fullCaseXS-loop-invariant
-                    this g sbH p vb vbl vbr)
-              (equal (acl2::sbyte32-fix p)
-                     (- (e (v-dp this)) (+ (H (dp)) (!q  (v-dp this) (dp))))))
-     :enable v-dp)
-   (defrule valueOfShiftLeft-!s_i-p-when-DoubleToDecimal.fullCaseXS-loop-invariant
-     (implies (DoubleToDecimal.fullCaseXS-loop-invariant
-                    this g sbH p vb vbl vbr)
-              (equal (Natural.valueOfShiftLeft (!s_i (i-dp g) (v-dp this) (dp)) p)
-                     (!u_i (i-dp g) (v-dp this) (dp))))
-     :enable (!u_i !s_i S v-dp)
-;     :enable (Natural.valueOfShiftLeft !u_i u_i !s_i S)
-;     :disable acl2::loghead
-     )
-|#
-     )
- )
-|#
-#|
-(defrulel aaaaaaa
-  (implies (DoubleToDecimal.fullCaseXS-loop-invariant
-            this g sbH p vb vbl vbr)
-           (acl2::sbyte64p sbH))
-  :use DoubleToDecimal.fullCaseXS-loop-invariant
-
-  )
-
-(defrule e-linear-dp
-   (implies (finite-positive-binary-p v (dp))
-            (and (<= (Emin (dp)) (e v))
-                 (<= (e v) (Emax (dp)))))
-   :rule-classes :linear
-   :use (:instance e-range-when-finite-positive-binary
-                   (f (dp))))
-
-(acl2::with-arith5-help
-(defrule p-fits-in-sbyte32
-   (implies (finite-positive-binary-p v (dp))
-            (acl2::sbyte32p
-             (+ (- (h (dp)))
-                (e v)
-                (- (!q v (dp))))))
-   :enable ((dp))))
-|#
-(local
- (acl2::with-arith5-help
-  (acl2::defrule loop-measure-decreases
+  (defrule loop-measure-decreases
     (implies (and (acl2::sbyte32p g)
                   (<= 0 g))
              (< (int-fix (+ -1 g)) g))
     :enable int-fix)))
 
 (acl2::with-arith5-help
- (acl2::define DoubleToDecimal.fullCaseXS-loop
+ (define DoubleToDecimal.fullCaseXS-loop
   ((this DoubleToDecimal-p)
    (g acl2::sbyte32p)
    (sbH acl2::sbyte64p)
