acl2/m5-lemmas.lisp
@@ -1,0 +1,836 @@
+#|
+(include-book "rtl/rel11/portcullis" :dir :system)
+(defpkg "LABEL" '(nil t))
+(defpkg "JVM" '(nil t))
+(DEFPKG "M5"
+  (set-difference-equal
+   (union-eq '(JVM::SCHEDULED
+               JVM::UNSCHEDULED
+               JVM::REF
+               JVM::LOCKED
+               JVM::S_LOCKED
+               JVM::UNLOCKED
+               JVM::AALOAD
+               JVM::AASTORE
+               JVM::ACONST_NULL
+               JVM::ALOAD
+               JVM::ALOAD_0
+               JVM::ALOAD_1
+               JVM::ALOAD_2
+               JVM::ALOAD_3
+               JVM::ANEWARRAY
+               JVM::ARETURN
+               JVM::ARRAYLENGTH
+               JVM::ASTORE
+               JVM::ASTORE_0
+               JVM::ASTORE_1
+               JVM::ASTORE_2
+               JVM::ASTORE_3
+               JVM::BALOAD
+               JVM::BASTORE
+               JVM::BIPUSH
+               JVM::CALOAD
+               JVM::CASTORE
+               JVM::DUP
+               JVM::DUP_X1
+               JVM::DUP_X2
+               JVM::DUP2
+               JVM::DUP2_X1
+               JVM::DUP2_X2
+               JVM::GETFIELD
+               JVM::GETSTATIC
+               JVM::GOTO
+               JVM::GOTO_W
+               JVM::I2B
+               JVM::I2C
+               JVM::I2L
+               JVM::I2S
+               JVM::IADD
+               JVM::IALOAD
+               JVM::IAND
+               JVM::IASTORE
+               JVM::ICONST_M1
+               JVM::ICONST_0
+               JVM::ICONST_1
+               JVM::ICONST_2
+               JVM::ICONST_3
+               JVM::ICONST_4
+               JVM::ICONST_5
+               JVM::IDIV
+               JVM::IF_ACMPEQ
+               JVM::IF_ACMPNE
+               JVM::IF_ICMPEQ
+               JVM::IF_ICMPGE
+               JVM::IF_ICMPGT
+               JVM::IF_ICMPLE
+               JVM::IF_ICMPLT
+               JVM::IF_ICMPNE
+               JVM::IFEQ
+               JVM::IFGE
+               JVM::IFGT
+               JVM::IFLE
+               JVM::IFLT
+               JVM::IFNE
+               JVM::IFNONNULL
+               JVM::IFNULL
+               JVM::IINC
+               JVM::ILOAD
+               JVM::ILOAD_0
+               JVM::ILOAD_1
+               JVM::ILOAD_2
+               JVM::ILOAD_3
+               JVM::IMUL
+               JVM::INEG
+               JVM::INSTANCEOF
+               JVM::INVOKESPECIAL
+               JVM::INVOKESTATIC
+               JVM::INVOKEVIRTUAL
+               JVM::IOR
+               JVM::IREM
+               JVM::IRETURN
+               JVM::ISHL
+               JVM::ISHR
+               JVM::ISTORE
+               JVM::ISTORE_0
+               JVM::ISTORE_1
+               JVM::ISTORE_2
+               JVM::ISTORE_3
+               JVM::ISUB
+               JVM::IUSHR
+               JVM::IXOR
+               JVM::JSR
+               JVM::JSR_W
+               JVM::L2I
+               JVM::LADD
+               JVM::LALOAD
+               JVM::LAND
+               JVM::LASTORE
+               JVM::LCMP
+               JVM::LCONST_0
+               JVM::LCONST_1
+               JVM::LDC
+               JVM::LDC_W
+               JVM::LDC2_W
+               JVM::LDIV
+               JVM::LLOAD
+               JVM::LLOAD_0
+               JVM::LLOAD_1
+               JVM::LLOAD_2
+               JVM::LLOAD_3
+               JVM::LMUL
+               JVM::LNEG
+               JVM::LOR
+               JVM::LREM
+               JVM::LRETURN
+               JVM::LSHL
+               JVM::LSHR
+               JVM::LSTORE
+               JVM::LSTORE_0
+               JVM::LSTORE_1
+               JVM::LSTORE_2
+               JVM::LSTORE_3
+               JVM::LSUB
+               JVM::LUSHR
+               JVM::LXOR
+               JVM::MONITORENTER
+               JVM::MONITOREXIT
+               JVM::MULTIANEWARRAY
+               JVM::NEW
+               JVM::NEWARRAY
+               JVM::NOP
+               JVM::POP
+               JVM::POP2
+               JVM::PUTFIELD
+               JVM::PUTSTATIC
+               JVM::RET
+               JVM::RETURN
+               JVM::SALOAD
+               JVM::SASTORE
+               JVM::SIPUSH
+               JVM::SWAP
+               ASSOC-EQUAL LEN NTH ZP SYNTAXP
+               QUOTEP FIX NFIX E0-ORDINALP E0-ORD-<)
+             (union-eq *acl2-exports*
+                       *common-lisp-symbols-from-main-lisp-package*))
+   '(PC PROGRAM PUSH POP RETURN REVERSE STEP ++)))
+|#
+(in-package "M5")
+(include-book "std/util/defredundant" :dir :system)
+(include-book "ihs/basic-definitions" :dir :system)
+(include-book "kestrel/utilities/fixbytes/instances" :dir :system)
+(include-book "rtl/rel11/support/excps" :dir :system)
+
+(include-book "tools/with-arith5-help" :dir :system)
+(local (acl2::allow-arith5-help))
+
+(acl2::define heap-ref-p (x)
+  :returns (yes booleanp :rule-classes ())
+  (and (consp x)
+       (equal (car x) 'ref)
+       (consp (cdr x))
+       (integerp (cadr x))
+       (<= -1 (cadr x))
+       (null (cddr x))))
+
+(acl2::define heap-ref-fix
+  ((x heap-ref-p))
+  :returns (x heap-ref-p)
+  (mbe :logic (if (heap-ref-p x) x (list 'ref -1))
+       :exec x)
+  ///
+  (acl2::defrule heap-ref-fix-when-heap-ref-p
+    (implies (heap-ref-p x)
+             (equal (heap-ref-fix x) x)))
+  (fty::deffixtype heap-ref
+    :pred heap-ref-p
+    :fix heap-ref-fix
+    :equiv heap-ref-equiv
+    :define t))
+
+(fty::defflexsum math.DoubleToDecimal
+  (:flds
+   :shape (and (true-listp x)
+               (equal (len x) 2)
+               (true-listp (car x))
+               (equal (len (car x)) 8)
+               (equal (car (car x)) "math.DoubleToDecimal")
+               (consp (cadr (car x)))
+               (equal (car (cadr (car x))) "e")
+               (consp (caddr (car x)))
+               (equal (car (caddr (car x))) "q")
+               (consp (cadddr (car x)))
+               (equal (car (cadddr (car x))) "c")
+               (consp (car (cddddr (car x))))
+               (equal (car (car (cddddr (car x)))) "lout")
+               (consp (cadr (cddddr (car x))))
+               (equal (car (cadr (cddddr (car x)))) "rout")
+               (consp (caddr (cddddr (car x))))
+               (equal (car (caddr (cddddr (car x)))) "buf")
+               (consp (cadddr (cddddr (car x))))
+               (equal (car (cadddr (cddddr (car x)))) "index")
+               (equal (cadr x)
+                      '("java.lang.Object" ("monitor" . 0)
+                        ("mcount" . 0)
+                        ("wait-set" . 0))))
+   :fields
+   ((e :type acl2::sbyte32 :acc-body (cdr (cadr (car x))))
+    (q :type acl2::sbyte32 :acc-body (cdr (caddr (car x))))
+    (c :type acl2::sbyte64 :acc-body (cdr (cadddr (car x))))
+    (lout :type acl2::sbyte32 :acc-body (cdr (car (cddddr (car x)))))
+    (rout :type acl2::sbyte32 :acc-body (cdr (cadr (cddddr (car x)))))
+    (buf :type heap-ref :acc-body (cdr (caddr (cddddr (car x)))))
+    (index :type acl2::sbyte32 :acc-body (cdr (cadddr (cddddr (car x))))))
+   :ctor-body (list
+               (list
+                "math.DoubleToDecimal"
+                (cons "e" e)
+                (cons "q" q)
+                (cons "c" c)
+                (cons "lout" lout)
+                (cons "rout" rout)
+                (cons "buf" buf)
+                (cons "index" index))
+               '("java.lang.Object" ("monitor" . 0)
+                 ("mcount" . 0)
+                 ("wait-set" . 0)))))
+
+(acl2::rule
+ (equal (math.DoubleToDecimal-kind x) :flds))
+
+(encapsulate ()
+  (local (include-book "models/jvm/m5/m5" :dir :system))
+
+  (verify-guards acl2::limitpart)
+  (verify-guards acl2::count2)
+  (verify-guards acl2::padd)
+  (verify-guards acl2::pmult)
+  (verify-guards acl2::ob*)
+  (verify-guards acl2::o-)
+  (verify-guards acl2::o^1)
+  (verify-guards acl2::o^2)
+  (verify-guards acl2::o^3h)
+  (verify-guards acl2::o^3)
+  (verify-guards acl2::o^4)
+  (verify-guards acl2::ob^)
+  (std::defredundant
+   :names (acl2::ob*
+           acl2::ob^
+           acl2::d<
+           acl2::lexp
+           acl2::l<
+           acl2::lsttoo
+           acl2::ltoo
+           acl2::well-founded-l<
+
+           push
+           top
+           pop
+           popn
+           bound?
+           bind
+           binding
+           op-code
+           arg1
+           arg2
+           arg3
+           nullrefp
+           reverse
+           *largest-integer-value*
+           *largest-long-value*
+           *most-negative-integer*
+           *most-negative-long*
+           u-fix
+           s-fix
+           byte-fix
+           ubyte-fix
+           short-fix
+           int-fix
+           uint-fix
+           long-fix
+           ulong-fix
+           char-fix
+           6-bit-fix
+           5-bit-fix
+           expt2
+           shl
+           shr
+           *mxcsr*
+           int2fp
+           fp2fp
+           fp2int
+           fpcmp
+           fp-binary
+           fpadd
+           fpsub
+           fpmul
+           fpdiv
+           fprem
+           fpneg
+           fpsqrt
+           bits2fp
+           make-state
+           thread-table
+           heap
+           class-table
+           make-thread
+           call-stack
+           status
+           rref
+           make-class-decl
+           class-decl-name
+           class-decl-superclasses
+           class-decl-fields
+           class-decl-sfields
+           class-decl-cp
+           class-decl-methods
+           class-decl-heapref
+           base-class-def
+           make-class-def
+           cp-make-double-entry
+           cp-make-float-entry
+           cp-make-int-entry
+           cp-make-long-entry
+           cp-string-resolved?
+           retrieve-cp
+           update-ct-string-ref
+           make-tt
+           addto-tt
+           mod-thread-scheduling
+           schedule-thread
+           unschedule-thread
+           rrefToThread
+           in-list
+           isThreadObject?
+           lock-object
+           unlock-object
+           objectlockable?
+           objectUnLockable?
+           make-frame
+           top-frame
+           pc
+           locals
+           stack
+           program
+           sync-flg
+           cur-class
+           method-name
+           method-formals
+           method-sync
+           method-program
+           method-isNative?
+           suppliedp
+           actual
+           modify
+           deref
+           field-value
+           build-class-field-bindings
+           build-class-object-field-bindings
+           build-immediate-instance-data
+           build-an-instance
+           build-class-data
+           build-a-class-instance
+           value-of
+           superclasses-of
+           array-content
+           array-type
+           array-bound
+           array-data
+           element-at
+           makearray
+           set-element-at
+           primitive-type
+           atype-to-identifier
+           identifier-to-atype
+           default-value1
+           init-array
+           natural-sum
+           makemultiarray2
+           makemultiarray
+           inst-length
+           execute-AALOAD
+           execute-AASTORE
+           execute-ACONST_NULL
+           execute-ALOAD
+           execute-ALOAD_X
+           execute-ANEWARRAY
+           execute-ARETURN
+           execute-ARRAYLENGTH
+           execute-ASTORE
+           execute-ASTORE_X
+           execute-BALOAD
+           execute-BASTORE
+           execute-BIPUSH
+           execute-CALOAD
+           execute-CASTORE
+           execute-D2F
+           execute-D2I
+           execute-D2L
+           execute-DADD
+           execute-DALOAD
+           execute-DASTORE
+           execute-DCMPG
+           execute-DCMPL
+           execute-DCONST_0
+           execute-DCONST_1
+           execute-DDIV
+           execute-DLOAD
+           execute-DLOAD_X
+           execute-DMUL
+           execute-DNEG
+           execute-DREM
+           execute-DRETURN
+           execute-DSTORE
+           execute-DSTORE_X
+           execute-DSUB
+           execute-DUP
+           execute-DUP_X1
+           execute-DUP_X2
+           execute-DUP2
+           execute-DUP2_X1
+           execute-DUP2_X2
+           execute-F2D
+           execute-F2I
+           execute-F2L
+           execute-FADD
+           execute-FALOAD
+           execute-FASTORE
+           execute-FCMPG
+           execute-FCMPL
+           execute-FCONST_0
+           execute-FCONST_1
+           execute-FCONST_2
+           execute-FDIV
+           execute-FLOAD
+           execute-FLOAD_X
+           execute-FMUL
+           execute-FNEG
+           execute-FREM
+           execute-FRETURN
+           execute-FSTORE
+           execute-FSTORE_X
+           execute-FSUB
+           execute-GETFIELD
+           static-field-value
+           execute-GETSTATIC
+           execute-GOTO
+           execute-GOTO_W
+           execute-I2B
+           execute-I2C
+           execute-I2D
+           execute-I2F
+           execute-I2L
+           execute-I2S
+           execute-IADD
+           execute-IALOAD
+           execute-IAND
+           execute-IASTORE
+           execute-ICONST_X
+           execute-IDIV
+           execute-IF_ACMPEQ
+           execute-IF_ACMPNE
+           execute-IF_ICMPEQ
+           execute-IF_ICMPGE
+           execute-IF_ICMPGT
+           execute-IF_ICMPLT
+           execute-IF_ICMPLE
+           execute-IF_ICMPNE
+           execute-IFEQ
+           execute-IFGE
+           execute-IFGT
+           execute-IFLE
+           execute-IFLT
+           execute-IFNE
+           execute-IFNONNULL
+           execute-IFNULL
+           execute-IINC
+           execute-ILOAD
+           execute-ILOAD_X
+           execute-IMUL
+           execute-INEG
+           execute-INSTANCEOF
+           execute-IOR
+           execute-IREM
+           execute-IRETURN
+           execute-ISHL
+           execute-ISHR
+           execute-ISTORE
+           execute-ISTORE_X
+           execute-ISUB
+           iushr
+           execute-IUSHR
+           execute-IXOR
+           execute-JSR
+           execute-JSR_W
+           class-name-of-ref
+           bind-formals
+           lookup-method-in-superclasses
+           lookup-method
+           execute-INVOKESPECIAL
+           execute-INVOKESTATIC
+           execute-INVOKEVIRTUAL
+           execute-L2D
+           execute-L2F
+           execute-L2I
+           execute-LADD
+           execute-LALOAD
+           execute-LAND
+           execute-LASTORE
+           execute-LCMP
+           execute-LCONST_X
+           set-instance-field
+           execute-LDC
+           execute-LDC2_W
+           execute-LDIV
+           execute-LLOAD
+           execute-LLOAD_X
+           execute-LMUL
+           execute-LNEG
+           execute-LOR
+           execute-LREM
+           execute-LRETURN
+           execute-LSHL
+           execute-LSHR
+           execute-LSTORE
+           execute-LSTORE_X
+           execute-LSUB
+           lushr
+           execute-LUSHR
+           execute-LXOR
+           execute-MONITORENTER
+           execute-MONITOREXIT
+           execute-MULTIANEWARRAY
+           execute-NEW
+           execute-NEWARRAY
+           execute-NOP
+           execute-POP
+           execute-POP2
+           execute-PUTFIELD
+           execute-PUTSTATIC
+           execute-RET
+           execute-RETURN
+           execute-SALOAD
+           execute-SASTORE
+           execute-SIPUSH
+           execute-SWAP
+           do-inst)))
+
+(acl2::defruled field-value-math.DoubleToDecimal
+ (acl2::b*
+  (((math.DoubleToDecimal-flds instance) instance))
+  (implies
+   (math.DoubleToDecimal-p instance)
+   (and
+    (equal (field-value "java.lang.Object" "monitor" instance)
+           0)
+    (equal (field-value "java.lang.Object" "mcount" instance)
+           0)
+    (equal (field-value "java.lang.Object" "wait-set" instance)
+           0)
+    (equal (field-value "math.DoubleToDecimal" "e" instance)
+           instance.e)
+    (equal (field-value "math.DoubleToDecimal" "q" instance)
+           instance.q)
+    (equal (field-value "math.DoubleToDecimal" "c" instance)
+           instance.c)
+    (equal (field-value "math.DoubleToDecimal" "lout" instance)
+           instance.lout)
+    (equal (field-value "math.DoubleToDecimal" "rout" instance)
+           instance.rout)
+    (equal (field-value "math.DoubleToDecimal" "buf" instance)
+           instance.buf)
+    (equal (field-value "math.DoubleToDecimal" "index" instance)
+           instance.index))))
+ :enable (math.DoubleToDecimal-p
+          math.DoubleToDecimal-flds->e
+          math.DoubleToDecimal-flds->q
+          math.DoubleToDecimal-flds->c
+          math.DoubleToDecimal-flds->lout
+          math.DoubleToDecimal-flds->rout
+          math.DoubleToDecimal-flds->buf
+          math.DoubleToDecimal-flds->index))
+
+(acl2::rule
+ (acl2::b*
+  ((top-frame (top-frame th s))
+   ((math.DoubleToDecimal-flds instance)
+    (deref (top (stack top-frame)) (heap s)))
+   (new-pc (+ 3 (pc top-frame)))
+   (stack (pop (stack top-frame))))
+  (implies
+   (and (math.DoubleToDecimal-p instance))
+   (and
+    (equal
+     (do-inst (list 'GETFIELD "java.lang.Object" "monitor" nil) th s)
+     (modify th s :pc new-pc
+             :stack (push 0 stack)))
+    (equal
+     (do-inst (list 'GETFIELD "java.lang.Object" "mcount" nil) th s)
+     (modify th s :pc new-pc
+             :stack (push 0 stack)))
+    (equal
+     (do-inst (list 'GETFIELD "java.lang.Object" "wait-set" nil) th s)
+     (modify th s :pc new-pc
+             :stack (push 0 stack)))
+    (equal
+     (do-inst (list 'GETFIELD "math.DoubleToDecimal" "e" nil) th s)
+     (modify th s :pc new-pc
+             :stack (push instance.e stack)))
+    (equal
+     (do-inst (list 'GETFIELD "math.DoubleToDecimal" "q" nil) th s)
+     (modify th s :pc new-pc
+             :stack (push instance.q stack)))
+    (equal
+     (do-inst (list 'GETFIELD "math.DoubleToDecimal" "c" t) th s)
+     (modify th s :pc new-pc
+             :stack (push 0 (push instance.c stack))))
+    (equal
+     (do-inst (list 'GETFIELD "math.DoubleToDecimal" "lout" nil) th s)
+     (modify th s :pc new-pc
+             :stack (push instance.lout stack)))
+    (equal
+     (do-inst (list 'GETFIELD "math.DoubleToDecimal" "rout" nil) th s)
+     (modify th s :pc new-pc
+             :stack (push instance.rout stack)))
+    (equal
+     (do-inst (list 'GETFIELD "math.DoubleToDecimal" "buf" t) th s)
+     (modify th s :pc new-pc
+             :stack (push 0 (push instance.buf stack))))
+    (equal
+     (do-inst (list 'GETFIELD "math.DoubleToDecimal" "index" nil) th s)
+     (modify th s :pc new-pc
+             :stack (push instance.index stack))))))
+ :enable field-value-math.DoubleToDecimal
+ :disable field-value)
+
+(acl2::defruled set-instance-field-math.DoubleToDecimal
+ (acl2::b*
+  (((math.DoubleToDecimal-flds i) instance))
+  (implies
+   (math.DoubleToDecimal-p instance)
+   (and
+    (implies
+     (acl2::sbyte32p e)
+     (equal (set-instance-field "math.DoubleToDecimal" "e" e instance)
+            (math.DoubleToDecimal-flds
+             e i.q i.c i.lout i.rout i.buf i.index)))
+    (implies
+     (acl2::sbyte32p q)
+     (equal (set-instance-field "math.DoubleToDecimal" "q" q instance)
+            (math.DoubleToDecimal-flds
+             i.e q i.c i.lout i.rout i.buf i.index)))
+    (implies
+     (acl2::sbyte64p c)
+     (equal (set-instance-field "math.DoubleToDecimal" "c" c instance)
+            (math.DoubleToDecimal-flds
+             i.e i.q c i.lout i.rout i.buf i.index)))
+    (implies
+     (acl2::sbyte32p lout)
+     (equal (set-instance-field "math.DoubleToDecimal" "lout" lout instance)
+            (math.DoubleToDecimal-flds
+             i.e i.q i.c lout i.rout i.buf i.index)))
+    (implies
+     (acl2::sbyte32p rout)
+     (equal (set-instance-field "math.DoubleToDecimal" "rout" rout instance)
+            (math.DoubleToDecimal-flds
+             i.e i.q i.c i.lout rout i.buf i.index)))
+    (implies
+     (heap-ref-p buf)
+     (equal (set-instance-field "math.DoubleToDecimal" "buf" buf instance)
+            (math.DoubleToDecimal-flds
+             i.e i.q i.c i.lout i.rout buf i.index)))
+    (implies
+     (acl2::sbyte32p index)
+     (equal (set-instance-field "math.DoubleToDecimal" "index" index instance)
+            (math.DoubleToDecimal-flds
+             i.e i.q i.c i.lout i.rout i.buf index))))))
+ :enable (math.DoubleToDecimal-p
+          math.DoubleToDecimal-flds->e
+          math.DoubleToDecimal-flds->q
+          math.DoubleToDecimal-flds->c
+          math.DoubleToDecimal-flds->lout
+          math.DoubleToDecimal-flds->rout
+          math.DoubleToDecimal-flds->buf
+          math.DoubleToDecimal-flds->index))
+
+(acl2::rule
+ (acl2::b*
+  ((top-frame (top-frame th s))
+   (stack (stack top-frame))
+   (heap (heap s))
+   (new-pc (+ 3 (pc top-frame))))
+  (and
+   (acl2::b*
+    ((e (top stack))
+     (ref (top (pop stack)))
+     (stack (pop (pop stack)))
+     (address (cadr ref))
+     ((math.DoubleToDecimal-flds i) (deref ref heap)))
+    (implies
+     (and (math.DoubleToDecimal-p i)
+          (acl2::sbyte32p e))
+     (and
+      (equal
+       (do-inst (list 'PUTFIELD "math.DoubleToDecimal" "e" nil) th s)
+       (modify th s :pc new-pc :stack stack
+               :heap (bind address
+                           (math.DoubleToDecimal-flds
+                            e i.q i.c i.lout i.rout i.buf i.index)
+                           heap))))))
+   (acl2::b*
+    ((q (top stack))
+     (ref (top (pop stack)))
+     (stack (pop (pop stack)))
+     (address (cadr ref))
+     ((math.DoubleToDecimal-flds i) (deref ref heap)))
+    (implies
+     (and (math.DoubleToDecimal-p i)
+          (acl2::sbyte32p q))
+     (and
+      (equal
+       (do-inst (list 'PUTFIELD "math.DoubleToDecimal" "q" nil) th s)
+       (modify th s :pc new-pc :stack stack
+               :heap (bind address
+                           (math.DoubleToDecimal-flds
+                            i.e q i.c i.lout i.rout i.buf i.index)
+                           heap))))))
+   (acl2::b*
+    ((c (top (pop stack)))
+     (ref (top (pop (pop stack))))
+     (stack (pop (pop (pop stack))))
+     (address (cadr ref))
+     ((math.DoubleToDecimal-flds i) (deref ref heap)))
+    (implies
+     (and (math.DoubleToDecimal-p i)
+          (acl2::sbyte64p c))
+     (and
+      (equal
+       (do-inst (list 'PUTFIELD "math.DoubleToDecimal" "c" t) th s)
+       (modify th s :pc new-pc :stack stack
+               :heap (bind address
+                           (math.DoubleToDecimal-flds
+                            i.e i.q c i.lout i.rout i.buf i.index)
+                           heap))))))
+   (acl2::b*
+    ((lout (top stack))
+     (ref (top (pop stack)))
+     (stack (pop (pop stack)))
+     (address (cadr ref))
+     ((math.DoubleToDecimal-flds i) (deref ref heap)))
+    (implies
+     (and (math.DoubleToDecimal-p i)
+          (acl2::sbyte32p lout))
+     (and
+      (equal
+       (do-inst (list 'PUTFIELD "math.DoubleToDecimal" "lout" nil) th s)
+       (modify th s :pc new-pc :stack stack
+               :heap (bind address
+                           (math.DoubleToDecimal-flds
+                            i.e i.q i.c lout i.rout i.buf i.index)
+                           heap))))))
+   (acl2::b*
+    ((rout (top stack))
+     (ref (top (pop stack)))
+     (stack (pop (pop stack)))
+     (address (cadr ref))
+     ((math.DoubleToDecimal-flds i) (deref ref heap)))
+    (implies
+     (and (math.DoubleToDecimal-p i)
+          (acl2::sbyte32p rout))
+     (and
+      (equal
+       (do-inst (list 'PUTFIELD "math.DoubleToDecimal" "rout" nil) th s)
+       (modify th s :pc new-pc :stack stack
+               :heap (bind address
+                           (math.DoubleToDecimal-flds
+                            i.e i.q i.c i.lout rout i.buf i.index)
+                           heap))))))
+   (acl2::b*
+    ((buf (top (pop stack)))
+     (ref (top (pop (pop stack))))
+     (stack (pop (pop (pop stack))))
+     (address (cadr ref))
+     ((math.DoubleToDecimal-flds i) (deref ref heap)))
+    (implies
+     (and (math.DoubleToDecimal-p i)
+          (heap-ref-p buf))
+     (and
+      (equal
+       (do-inst (list 'PUTFIELD "math.DoubleToDecimal" "buf" t) th s)
+       (modify th s :pc new-pc :stack stack
+               :heap (bind address
+                           (math.DoubleToDecimal-flds
+                            i.e i.q i.c i.lout i.rout buf i.index)
+                           heap))))))
+   (acl2::b*
+    ((index (top stack))
+     (ref (top (pop stack)))
+     (stack (pop (pop stack)))
+     (address (cadr ref))
+     ((math.DoubleToDecimal-flds i) (deref ref heap)))
+    (implies
+     (and (math.DoubleToDecimal-p i)
+          (acl2::sbyte32p index))
+     (and
+      (equal
+       (do-inst (list 'PUTFIELD "math.DoubleToDecimal" "index" nil) th s)
+       (modify th s :pc new-pc :stack stack
+               :heap (bind address
+                           (math.DoubleToDecimal-flds
+                            i.e i.q i.c i.lout i.rout i.buf index)
+                           heap))))))))
+ :enable set-instance-field-math.DoubleToDecimal
+ :disable set-instance-field
+ :prep-lemmas
+ ((acl2::defrule popn-2
+    (equal (popn 2 stack)
+           (cddr stack)))))
+
+(defconst *math.DoubleToDecimal-class-stub*
+   (make-class-decl
+    "math.DoubleToDecimal"
+    '("java.lang.Object")
+    '("e" "q" "c" "lout" "rout" "buf" "index")
+    '("LTR" "MASK_LTR" "MASK_SIGNIFICAND" "D" "threadLocal")
+    ()
+    ()
+    '(REF -1)))
